com.io7m.calino.specification/src/main/rocq/Calino/ThreeDMipMap.v
@@ -1,0 +1,265 @@
+(*
+ * Copyright © 2026 Mark Raynsford <code@io7m.com> https://www.io7m.com
+ *
+ * Permission to use, copy, modify, and/or distribute this software for any
+ * purpose with or without fee is hereby granted, provided that the above
+ * copyright notice and this permission notice appear in all copies.
+ *
+ * THE SOFTWARE IS PROVIDED "AS IS" AND THE AUTHOR DISCLAIMS ALL WARRANTIES
+ * WITH REGARD TO THIS SOFTWARE INCLUDING ALL IMPLIED WARRANTIES OF
+ * MERCHANTABILITY AND FITNESS. IN NO EVENT SHALL THE AUTHOR BE LIABLE FOR ANY
+ * SPECIAL, DIRECT, INDIRECT, OR CONSEQUENTIAL DAMAGES OR ANY DAMAGES
+ * WHATSOEVER RESULTING FROM LOSS OF USE, DATA OR PROFITS, WHETHER IN AN
+ * ACTION OF CONTRACT, NEGLIGENCE OR OTHER TORTIOUS ACTION, ARISING OUT OF OR
+ * IN CONNECTION WITH THE USE OR PERFORMANCE OF THIS SOFTWARE.
+ *)
+
+From Stdlib Require Import Arith.PeanoNat.
+From Stdlib Require Import Lists.List.
+From Stdlib Require Import Init.Nat.
+From Stdlib Require Import Bool.Bool.
+
+Require Import com.io7m.calino.ImageSize.
+
+Import ListNotations.
+
+Inductive threeDMipMapIndexT : Set := ThreeDMipMapIndex {
+  threeDMipMapLevel : nat;
+  threeDMipMapDepth : nat;
+}.
+
+Inductive threeDMipMapIndexOrd : threeDMipMapIndexT -> threeDMipMapIndexT -> Prop :=
+  | ThreeDMMIOrdEq : forall i0 i1,
+    i0 = i1 -> threeDMipMapIndexOrd i0 i1
+  | ThreeDMMIOrdLevelEq : forall i0 i1,
+    threeDMipMapLevel i0 = threeDMipMapLevel i1 ->
+      threeDMipMapDepth i0 < threeDMipMapDepth i1 ->
+        threeDMipMapIndexOrd i0 i1
+  | ThreeDMMIOrdLevelLt : forall i0 i1,
+    threeDMipMapLevel i1 < threeDMipMapLevel i0 ->
+      threeDMipMapIndexOrd i0 i1.
+
+Inductive threeDMipMapIndicesSorted : list threeDMipMapIndexT -> Prop :=
+  | ThreeDMMIOne  : forall m, threeDMipMapIndicesSorted [m]
+  | ThreeDMMICons : forall mmx mmy mxs,
+    threeDMipMapIndexOrd mmx mmy ->
+      threeDMipMapIndicesSorted (mmy :: mxs) ->
+        threeDMipMapIndicesSorted (mmx :: mmy :: mxs).
+
+Inductive threeDMipMap : Set := ThreeDMipMap {
+  threeDMipMapIndex            : threeDMipMapIndexT;
+  threeDMipMapOffset           : nat;
+  threeDMipMapSizeCompressed   : nat;
+  threeDMipMapSizeUncompressed : nat;
+  threeDMipMapCRC32            : nat
+}.
+
+Inductive threeDMipMapOffsetsSorted : list threeDMipMap -> Prop :=
+  | ThreeDMMSizeOne  : forall m, threeDMipMapOffsetsSorted [m]
+  | ThreeDMMSizeCons : forall mm0 mm1 mxs,
+    ((threeDMipMapOffset mm1) + (threeDMipMapSizeCompressed mm1)) < (threeDMipMapOffset mm0) ->
+      threeDMipMapOffsetsSorted (mm0 :: mxs) ->
+        threeDMipMapOffsetsSorted (mm1 :: mm0 :: mxs).
+
+Fixpoint threeDMipMapDepthCountForLevel
+  (level : nat)
+  (m     : list threeDMipMap)
+: nat :=
+  match m with
+  | []        => 0
+  | (x :: xs) =>
+    match Nat.eq_dec (threeDMipMapLevel (threeDMipMapIndex x)) level with
+    | left _  => 1 + (threeDMipMapDepthCountForLevel level xs)
+    | right _ => (threeDMipMapDepthCountForLevel level xs)
+    end
+  end.
+
+Definition threeDMipMapLevels (m : list threeDMipMap) : list nat :=
+  nodup Nat.eq_dec (map (fun k => threeDMipMapLevel (threeDMipMapIndex k)) m).
+
+Definition threeDMipMapsHaveSameDepths : (list threeDMipMap) -> nat -> nat -> Prop :=
+  fun m level0 level1 =>
+    In level0 (threeDMipMapLevels m) ->
+      In level1 (threeDMipMapLevels m) ->
+        threeDMipMapDepthCountForLevel level0 m = threeDMipMapDepthCountForLevel level1 m.
+
+Inductive threeDMipMapList : Set := ThreeDMipMapList {
+  threeDMipMaps                : list threeDMipMap;
+  threeDMipMapIndicesAreSorted : threeDMipMapIndicesSorted (map threeDMipMapIndex threeDMipMaps);
+  threeDMipMapOffsetAreSorted  : threeDMipMapOffsetsSorted threeDMipMaps;
+  threeDMipMapSameDepths       : forall level0 level1, threeDMipMapsHaveSameDepths threeDMipMaps level0 level1
+}.
+
+Inductive threeDMipMapImageSize : Set := ThreeDMipMapImageSize {
+  threeDSizeX      : nat;
+  threeDSizeY      : nat;
+  threeDSizeZ      : nat;
+  threeDSizeXRange : 1 < threeDSizeX;
+  threeDSizeYRange : 1 < threeDSizeY;
+  threeDSizeZRange : 1 < threeDSizeZ;
+}.
+
+Lemma threeDMipMapsNonEmpty : forall (m : threeDMipMapList),
+  [] <> threeDMipMaps m.
+Proof.
+  intros m.
+  destruct (threeDMipMapOffsetAreSorted m).
+  - discriminate.
+  - discriminate.
+Qed.
+
+Definition threeDMipMapFirst (m : threeDMipMapList) : threeDMipMap.
+Proof.
+  assert ([] <> threeDMipMaps m) as Hneq by (apply (threeDMipMapsNonEmpty)).
+  destruct (threeDMipMaps m) eqn:Hm.
+  - contradiction.
+  - exact t.
+Defined.
+
+Lemma lt_neq : forall n, 0 <> n <-> 0 < n.
+Proof.
+  intros n.
+  constructor.
+  - intro Hneq.
+    induction n as [|k].
+    -- unfold not in Hneq.
+       assert (0 = 0) as Heq by reflexivity.
+       contradiction.
+    -- apply (Nat.lt_0_succ k).
+  - intro Hneq.
+    induction n as [|k].
+    -- inversion Hneq.
+    -- discriminate.
+Qed.
+
+Lemma lt_neq_0 : forall n, 0 <> n -> 0 < n.
+Proof.
+  intros n Hneq.
+  rewrite <- lt_neq; trivial.
+Qed.
+
+Lemma lt_neq_1 : forall n, 0 < n -> 0 <> n.
+Proof.
+  intros n Hneq.
+  rewrite lt_neq; trivial.
+Qed.
+
+Definition threeDMipMapSize
+  (level      : nat)
+  (imageSize  : imageSize3D)
+  (levelRange : 0 < level)
+: option threeDMipMapImageSize :=
+  let sx  := (sizeX imageSize) / 2 ^ level  in
+  let sy  := (sizeY imageSize) / 2 ^ level  in
+  let sz  := (sizeZ imageSize) / 2 ^ level  in
+    match (Nat.ltb_spec0 1 sx, Nat.ltb_spec0 1 sy, Nat.ltb_spec0 1 sz) with
+    | (ReflectT _ xt, ReflectT _ yt, ReflectT _ zt) => Some (ThreeDMipMapImageSize sx sy sz xt yt zt)
+    | (_, _, _)                                     => None
+    end.
+
+Fixpoint threeDMipMapImageDataSizeTotalAux (m : list threeDMipMap) : nat :=
+  match m with
+  | []        => 0
+  | (x :: []) => (threeDMipMapOffset x) + (threeDMipMapSizeCompressed x)
+  | (x :: xs) => threeDMipMapImageDataSizeTotalAux xs
+  end.
+
+Definition threeDMipMapImageDataSizeTotal (m : threeDMipMapList) : nat :=
+  threeDMipMapImageDataSizeTotalAux (threeDMipMaps m).
+
+Example exampleThreeDMipMapsIndices := [
+  (ThreeDMipMapIndex 2 0);
+  (ThreeDMipMapIndex 2 1);
+  (ThreeDMipMapIndex 2 2);
+  (ThreeDMipMapIndex 1 0);
+  (ThreeDMipMapIndex 1 1);
+  (ThreeDMipMapIndex 1 2);
+  (ThreeDMipMapIndex 0 0);
+  (ThreeDMipMapIndex 0 1);
+  (ThreeDMipMapIndex 0 2)
+].
+
+Example exampleThreeDMipMaps :=
+  map (fun i => ThreeDMipMap i 0 0 0 0) exampleThreeDMipMapsIndices.
+
+Example exampleThreeDMipMapIndicesSorted : threeDMipMapIndicesSorted exampleThreeDMipMapsIndices.
+Proof.
+  apply ThreeDMMICons. { apply ThreeDMMIOrdLevelEq. reflexivity. compute; constructor. }
+  apply ThreeDMMICons. { apply ThreeDMMIOrdLevelEq. reflexivity. compute; constructor. }
+  apply ThreeDMMICons. { apply ThreeDMMIOrdLevelLt. compute; constructor. }
+  apply ThreeDMMICons. { apply ThreeDMMIOrdLevelEq. reflexivity. compute; constructor. }
+  apply ThreeDMMICons. { apply ThreeDMMIOrdLevelEq. reflexivity. compute; constructor. }
+  apply ThreeDMMICons. { apply ThreeDMMIOrdLevelLt. compute; constructor. }
+  apply ThreeDMMICons. { apply ThreeDMMIOrdLevelEq. reflexivity. compute; constructor. }
+  apply ThreeDMMICons. { apply ThreeDMMIOrdLevelEq. reflexivity. compute; constructor. }
+  apply ThreeDMMIOne.
+Qed.
+
+Example exampleThreeDMipMapsHaveSameDepths0 : threeDMipMapDepthCountForLevel 0 exampleThreeDMipMaps = 3.
+Proof. reflexivity. Qed.
+Example exampleThreeDMipMapsHaveSameDepths1 : threeDMipMapDepthCountForLevel 1 exampleThreeDMipMaps = 3.
+Proof. reflexivity. Qed.
+Example exampleThreeDMipMapsHaveSameDepths2 : threeDMipMapDepthCountForLevel 2 exampleThreeDMipMaps = 3.
+Proof. reflexivity. Qed.
+
+Example exampleThreeDMipMapsLevel : forall n, In n (threeDMipMapLevels exampleThreeDMipMaps) ->
+  n = 0 \/ n = 1 \/ n = 2.
+Proof.
+  intros n.
+  simpl.
+  intros H.
+  destruct H; auto.
+  destruct H; auto.
+  destruct H; auto.
+  contradiction H.
+Qed.
+
+Example exampleThreeDMipMapsHaveSameDepths : forall level0 level1, threeDMipMapsHaveSameDepths exampleThreeDMipMaps level0 level1.
+Proof.
+  intros level0 level1.
+  unfold threeDMipMapsHaveSameDepths.
+  intros H_In0 H_In1.
+  assert (level0 = 0 \/ level0 = 1 \/ level0 = 2) as Hl0 by (apply (exampleThreeDMipMapsLevel level0 H_In0)).
+  assert (level1 = 0 \/ level1 = 1 \/ level1 = 2) as Hl1 by (apply (exampleThreeDMipMapsLevel level1 H_In1)).
+  destruct Hl0 as [Heq0|Heq0]. {
+    destruct Hl1 as [Heq1|Heq1]. {
+      rewrite Heq0.
+      rewrite Heq1.
+      reflexivity.
+    }
+    destruct Heq1 as [Heq1_0|Heq1_0]. {
+      rewrite Heq0.
+      rewrite Heq1_0.
+      reflexivity.
+    }
+    rewrite Heq0.
+    rewrite Heq1_0.
+    reflexivity.
+  }
+  destruct Heq0 as [Heq0_0|Heq0_0]. {
+    rewrite Heq0_0.
+    destruct Hl1 as [Heq1|Heq1]. {
+      rewrite Heq1.
+      reflexivity.
+    }
+    destruct Heq1 as [Heq1_0|Heq1_0]. {
+      rewrite Heq1_0.
+      reflexivity.
+    }
+    rewrite Heq1_0.
+    reflexivity.
+  }
+  destruct Hl1 as [Heq1|Heq1]. {
+    rewrite Heq0_0.
+    rewrite Heq1.
+    reflexivity.
+  }
+  destruct Heq1 as [Heq1_0|Heq1_0]. {
+    rewrite Heq0_0.
+    rewrite Heq1_0.
+    reflexivity.
+  }
+  rewrite Heq0_0.
+  rewrite Heq1_0.
+  reflexivity.
+Qed.
